newest/stepWF.v
@@ -1,5 +1,5 @@
-Require Import SfLib.       
-Require Import NonSpec.  
+Require Import SfLib.           
+Require Import NonSpec.   
 Require Import Spec.  
 Require Import Coq.Sets.Ensembles. 
 Require Import erasure. 
@@ -8,18 +8,10 @@ Require Import hetList.
 Require Import Coq.Program.Equality. 
 Require Import unspec. 
 Require Import sets. 
-Require Import Heap. 
 Require Import classifiedStep. 
-Require Import Coq.Sets.Powerset_facts.
+Require Import Coq.Sets.Powerset_facts. 
+Require Import Heap. 
 (*Require Import ForkIndependence. *)
-
-Theorem destructEnd : forall (T:Type) (l : list T), l = [] \/ exists (a:T) l', l = l' ++ [a]. 
-Proof.
-  induction l. 
-  {auto. }
-  {inversion IHl. right. exists a. exists nil. simpl. subst. auto. 
-   inv H. inv H0. right. exists x. exists (a::x0). auto. }
-Qed. 
 
 Axiom uniqueTP : forall T1 T2 t, tIn (tUnion T1 T2) t -> tIn T1 t -> tIn T2 t -> False. 
 
@@ -35,80 +27,6 @@ Proof.
 Qed. 
 
 Hint Constructors Union Couple. 
-
-Theorem coupleUnion : forall X t1 t2, Couple X t1 t2 = Union X (Singleton X t1) (Singleton X t2). 
-Proof.
-  intros. apply Extensionality_Ensembles. unfold Same_set. unfold Included. split; intros. 
-  {inversion H; subst; auto. }
-  {inversion H; subst. inversion H0; subst; auto. inversion H0; subst; auto. }
-Qed. 
-
-Axiom moveToUnused : forall t T T' H H', 
-              multistep H tEmptySet (tUnion T (tSingleton t)) (OK H' tEmptySet (tUnion T' (tSingleton t))) <->
-              multistep H (tSingleton t) T (OK H' (tSingleton t) T'). 
-
-Ltac replaceWithEmpty :=
-  match goal with
-      |H:multistep ?H (tSingleton ?t) ?T ?x |- _ => 
-       let n := fresh in
-       assert(n:(tSingleton t) = tUnion (tSingleton t) tEmptySet) by (unfold tUnion; rewrite union_empty_r; auto)
-      | |-multistep ?H (tSingleton ?t) ?T ?x => 
-       let n := fresh in
-       assert(n:(tSingleton t) = tUnion (tSingleton t) tEmptySet) by (unfold tUnion; rewrite union_empty_r; auto)  
-  end. 
-
-Theorem raw_unspecHeapSpecWrite : forall H x s s1 M a c d TID tid' M',
-                raw_heap_lookup x H = Some (sfull (unlocked nil) s (aCons c d) tid' M')->
-                raw_unspecHeap (raw_replace x (sfull (unlocked nil) (Empty_set tid) (aCons a s1) TID M) H) = 
-                raw_unspecHeap H.
-Proof.
-  induction H; intros. 
-  {inv H. }
-  {simpl in *. destruct a. destruct (beq_nat x i) eqn:eq. 
-   {inv H0. simpl. apply beq_nat_true in eq. subst. destruct s1; simpl. destruct d; simpl. 
-    auto. auto. auto. destruct d; simpl; auto. destruct d; simpl; auto. }
-   {simpl. erewrite IHlist; eauto. }
-  }
-Qed. 
-
-Theorem unspecHeapSpecWrite : forall H x s s1 M a c d TID tid' M',
-                            heap_lookup x H = Some (sfull (unlocked nil) s (aCons c d) tid' M')->
-                            unspecHeap (replace x (sfull (unlocked nil) (Empty_set tid) (aCons a s1) TID M) H) =
-                            unspecHeap H.
-Proof.
-  intros. destruct H. apply rawHeapsEq. eapply raw_unspecHeapSpecWrite; eauto.
-Qed. 
-
-Theorem raw_lookupUnspecFull : forall H x ds t N, 
-                             raw_heap_lookup x H = Some(sfull (unlocked nil) ds (unlocked nil) t N) ->
-                             raw_heap_lookup x (raw_unspecHeap H) =
-                             Some(sfull (unlocked nil) (Empty_set tid) (unlocked nil) t N).
-Proof.
-  induction H; intros. 
-  {inv H. }
-  {simpl in *. destruct a. destruct (beq_nat x i) eqn:eq. 
-   {inv H0. simpl. rewrite eq. auto. }
-   {destruct i0. destruct (commit a); eauto. simpl. rewrite eq. eauto. destruct (commit a); eauto.
-    destruct (commit a0). simpl. rewrite eq. eauto. simpl. rewrite eq; eauto. }
-  }
-Qed. 
-
-Theorem lookupUnspecFull : forall H x ds t N, 
-                             heap_lookup x H = Some(sfull (unlocked nil) ds (unlocked nil) t N) ->
-                             heap_lookup x (unspecHeap H) = 
-                             Some(sfull (unlocked nil) (Empty_set tid) (unlocked nil) t N).
-Proof.
-  intros. destruct H. simpl. eapply raw_lookupUnspecFull; eauto.
-Qed. 
-
-Theorem listAlign2 : forall (T:Type) b a, exists (c : list T) d, a::b = c++[d]. 
-Proof.
-  induction b; intros. 
-  {eauto. }
-  {specialize (IHb a). invertHyp. rewrite H0. eauto. }
-Qed. 
-
-Ltac alignTac a b := assert(exists c d, a::b = c++[d]) by apply listAlign2; invertHyp.
 
 Ltac eUnspec :=
   match goal with
@@ -131,18 +49,7 @@ Theorem rollbackWF : forall H H' T TR TR' tidR acts,
                        wellFormed H' (tUnion T TR'). 
 Admitted. 
 
-Theorem spec_multi_trans : forall H H' H'' T T' T'',
-                        spec_multistep H T H' T' ->
-                        spec_multistep H' T' H'' T'' ->
-                        spec_multistep H T H'' T''.  
-Proof.
-  intros. genDeps {H''; T''}. induction H0; intros.  
-  {auto. }
-  {apply IHspec_multistep in H1. econstructor. eauto. auto. }
-Qed. 
-
 Hint Constructors spec_step. 
-
 
 Theorem UnionEqTID : forall T T' tid s1 s2 M s1' s2' M',
                        tUnion T (tSingleton(tid,s1,s2,M)) = tUnion T' (tSingleton(tid,s1',s2',M')) ->
@@ -184,22 +91,14 @@ Inductive eraseTrm : list action -> trm -> trm -> Prop :=
 |eraseTrmFork : forall t E M d N s, eraseTrm (s++[fAct t E M d]) N t
 |eraseTrmSR : forall t E M N d M' s, eraseTrm (s++[srAct t E M N d]) M' t. 
 
-Inductive unspecTrm : actionStack -> trm -> trm -> actionStack -> Prop :=
-|unspecUnlocked : forall s M M', eraseTrm s M M' -> unspecTrm (unlocked s) M M' (unlocked nil)
-|unspecSpecStack : forall s M N, unspecTrm (specStack s N) M N (specStack nil N). 
-
-Theorem unspecEraseTrm : forall tid s1 s1' s2 M M', 
-                          unspecTrm s1 M M' s1' ->
-                          unspecThread(tid,s1,s2,M) (tSingleton(tid,s1',s2,M')). 
+Theorem unspecEraseTrm : forall tid s1 s2 M M', 
+                          eraseTrm s1 M M' ->
+                          unspecThread(tid,unlocked s1,s2,M) (tSingleton(tid,unlocked nil,s2,M')). 
 Proof.
-  intros. destruct s1. 
-  {inv H. }
-  {destructLast l. 
-   {inv H. inv H1; try invertListNeq. auto. }
-   {invertHyp. inv H. destruct x; inv H1; try solve[invertListNeq]; apply lastElementEq in H0; 
-   inv H0; unspecThreadTac; auto. }
-  }
-  {destructLast l; inv H; auto. }
+  intros. destructLast s1. 
+   {inv H; try invertListNeq. auto. }
+   {invertHyp. inv H; try solve[invertListNeq]; apply lastElementEq in H1;
+   subst; unspecThreadTac; auto. }
 Qed. 
 
 Theorem eEraseTrm : forall s1 M, exists M', eraseTrm s1 M M'. 
@@ -210,12 +109,267 @@ Qed.
 
 Ltac eraseTrmTac s1 M := assert(exists M', eraseTrm s1 M M') by apply eEraseTrm; invertHyp.  
 
+Theorem EqJMeq : forall (T:Type) (x y:T), x = y -> JMeq x y.
+Proof.
+  intros. subst. auto. Qed. 
+
+Axiom UnionSingletonEq : forall T T' a b, 
+                 tUnion T (tSingleton a) = tUnion T' (tSingleton b) -> 
+                 tIn T' a -> T = tUnion (Subtract thread T' a) (tSingleton b).
+
+Ltac invertDecomp :=
+  match goal with
+    |H:(?a,?b,?c,?d)=(?e,?f,?g,?h) |- _ => inv H
+    |H:?x = ?y |- _ => solve[inv H]
+    |H:decompose ?M ?E ?e,H':decompose ?M' ?E' ?e' |- _=>
+     eapply uniqueCtxtDecomp in H; eauto; invertHyp
+  end. 
+
+Axiom UnionSingletonCoupleEq : forall T T' a b c, 
+                 tUnion T (tSingleton a) = tUnion T' (tCouple b c) -> 
+                 tIn T' a -> T = tUnion (Subtract thread T' a) (tCouple b c).
+
+Axiom CoupleUnionAx : forall T T' t1 t2,
+                        tUnion T (tSingleton t1) = tUnion T' (tCouple t1 t2) -> 
+                        T = tUnion T' (tSingleton t2). 
+
+
+Theorem simSpecJoin : forall H T H' T' tid s1 s2 M' M'',
+                        spec_multistep H (tUnion T (tSingleton(tid,s1,s2,M'))) H' 
+                                       (tUnion T' (tSingleton(tid,s1,s2,M''))) ->
+                        spec_multistep H T H' T'. 
+Proof.
+  intros. dependent induction H0. 
+  {unfoldTac. apply UnionEqTID in x. invertHyp. constructor. }
+  {copy x. unfoldSetEq x. copy H. apply specStepSingleton in H4. invertHyp. 
+   assert(tIn (tUnion T0 (tSingleton x)) x). apply Union_intror. constructor.
+   apply H2 in H4. inv H4. 
+   {copy H5. apply pullOut in H5. rewrite H5. econstructor. eapply specStepChangeUnused. 
+    eauto. eapply IHspec_multistep. Focus 2. auto. apply UnionSingletonEq in H1. rewrite H1. 
+    unfoldTac. rewrite UnionSwap. auto. auto. }
+   {inv H5. inv H. 
+    {unfoldTac; invertHyp. inv H4. eapply IHspec_multistep; eauto. apply UnionEqTID in H1. 
+     invertHyp. auto. }
+     {unfoldTac; invertHyp. inv H7. eapply monotonicActions in H0. Focus 2. 
+      apply Union_intror. constructor. Focus 2. apply Union_intror. constructor.
+      destruct s1; simpl in *; omega. }
+     {unfoldTac; invertHyp. inv H4. eapply monotonicActions in H0. Focus 2. 
+      apply Union_intror. constructor. Focus 2. apply Union_intror. constructor.
+      destruct s1; simpl in *; omega. }
+     {unfoldTac; invertHyp. inv H4. eapply monotonicActions in H0. Focus 2. 
+      apply Union_intror. constructor. Focus 2. apply Union_intror. constructor.
+      destruct s1; simpl in *; omega. }
+     {unfoldTac; invertHyp. inv H4. eapply monotonicActions in H0. Focus 2. 
+      apply Union_intror. constructor. Focus 2. apply Union_intror. constructor.
+      destruct s1; simpl in *; omega. }
+     {unfoldTac; invertHyp. inv H7. eapply monotonicActions in H0. Focus 2. 
+      apply Union_intror. constructor. Focus 2. apply Union_intror. constructor.
+      destruct s1; simpl in *; omega. }
+    }
+  }
+Qed. 
+
+Theorem wrapDistributeApp : forall s a N E e p, 
+                              wrapActs(s++[a]) N E e p = wrapActs(s) N E e p++ wrapActs[a] N E e p.
+Proof.
+  induction s; intros. 
+  {simpl. destruct a; auto. }
+  {simpl. destruct a; auto; destruct a0; auto; rewrite IHs; auto. }
+Qed. 
+
+Theorem wrapEraseTrm : forall s M M' N N' E p,
+                         eraseTrm s M M' -> 
+                         eraseTrm (wrapActs s N E N' p) 
+                                  (fill E (specJoin (ret N) M)) (fill E (specJoin (ret N) M')). 
+Proof.
+  intros. inv H; try solve[rewrite wrapDistributeApp; constructor]. 
+  {simpl. constructor. }
+Qed. 
+
+
+Ltac specActEq H := 
+  eapply firstSpecActEq in H; [idtac|apply Union_intror; rewrite app_nil_l; constructor|
+                               apply Union_intror; constructor]. 
+
+Theorem eraseTrmApp : forall x a M M', 
+                        eraseTrm (x ++ [a]) M M' -> actionTerm a M'. 
+Proof.
+  intros. inv H; try solve[apply lastElementEq in H1; subst; constructor].
+  invertListNeq. 
+Qed. 
+
+Theorem specFastForward : forall H T H' T' tid x0 x s2' N N0 M M' M'',
+             eraseTrm (x0++[x]) N M' ->                                                
+             spec_multistep H (tUnion T (tSingleton(tid,specStack nil N0, s2', M)))
+                            H' (tUnion T' (tSingleton(tid,specStack(x0++[x]) N0, s2', M''))) ->
+             exists H'' T'',
+               spec_multistep H (tUnion T (tSingleton(tid,specStack nil N0, s2', M))) 
+                              H'' (tUnion T'' (tSingleton(tid,specStack nil N0, s2', M'))) /\
+               spec_multistep H'' (tUnion T'' (tSingleton(tid, specStack nil N0, s2', M')))
+                              H' (tUnion T' (tSingleton(tid,specStack(x0++[x]) N0, s2',M''))). 
+Proof.
+  intros. dependent induction H1. 
+  {apply UnionEqTID in x. invertHyp. inv H. invertListNeq. }
+  {copy x. unfoldSetEq H2. copy H. apply specStepSingleton in H2. invertHyp. 
+   assert(tIn (tUnion T0 (tSingleton x2)) x2). apply Union_intror. constructor. apply H3 in H2. 
+   inv H2. 
+   {eapply IHspec_multistep in H0. Focus 3. auto. Focus 2. apply UnionSingletonEq in x; auto.  
+    rewrite x. unfoldTac. rewrite UnionSwap. auto. invertHyp. exists x3. exists x4. split; auto.
+    apply pullOut in H5. unfoldTac. rewrite H5. rewrite UnionSwap. econstructor. 
+    eapply specStepChangeUnused. eauto. unfoldTac. rewrite <- UnionSwap. eauto. }
+   {inv H5. apply UnionEqTID in x. invertHyp. clear H2 H5 H7. inversion H; subst. 
+    {unfoldTac; invertHyp. inv H2. eapply IHspec_multistep in H0. Focus 3. 
+     auto. Focus 2. auto. invertHyp. exists x. exists x2. split; eauto. econstructor. 
+     eapply SBasicStep; eauto. assumption. }
+    {unfoldTac; invertHyp. inv H7. copy H1. specActEq H1. subst. 
+     apply eraseTrmApp in H0. inv H0.  exists h'. exists T. split. constructor. 
+     econstructor. eapply SFork. eauto. }
+    {unfoldTac; invertHyp. inv H2. copy H1. specActEq H1. subst. exists h. exists T. 
+     apply eraseTrmApp in H0. inv H0. split. constructor. econstructor. 
+     eauto. eauto. }
+    {unfoldTac; invertHyp. inv H2. copy H1. specActEq H1. subst. exists h. exists T. 
+     apply eraseTrmApp in H0. inv H0. split. constructor. econstructor. 
+     eauto. eauto. }
+    {unfoldTac; invertHyp. inv H2. copy H1. specActEq H1. subst. exists h. exists T. 
+     apply eraseTrmApp in H0. inv H0. split. constructor. econstructor. 
+     eauto. eauto. }
+    {unfoldTac; invertHyp. inv H7. copy H1. specActEq H1. subst. apply eraseTrmApp in H0. 
+     inv H0. exists h'. exists T. split. constructor. econstructor. eauto. eauto. }
+   }
+  }
+Qed. 
+
+Ltac monoActs H :=
+  eapply monotonicActions in H;[idtac|apply Union_intror; constructor|apply Union_intror;constructor].
+
+Theorem simTSteps : forall H T H' T' tid s1 s2 s1' s2' N M M' tid',
+                      spec_multistep H (tUnion T (tSingleton(tid,s1,s2,M)))
+                                     H' (tUnion T' (tSingleton(tid,s1,s2,M'))) ->
+                      spec_multistep H (tUnion T (tSingleton(tid',s1',s2',N)))
+                                     H' (tUnion T' (tSingleton(tid',s1',s2',N))). 
+Proof.
+  intros. dependent induction H0. 
+  {apply UnionEqTID in x. invertHyp. constructor. }
+  {copy x. unfoldSetEq x. copy H. apply specStepSingleton in H4. invertHyp. 
+   assert(tIn (tUnion T0 (tSingleton x)) x). apply Union_intror. constructor. 
+   apply H2 in H4. inv H4. 
+   {copy H5. apply pullOut in H5. rewrite H5. unfoldTac. rewrite UnionSwap. econstructor. 
+    eapply specStepChangeUnused. eauto. unfoldTac. rewrite <- UnionSwap.
+    eapply IHspec_multistep; eauto. apply UnionSingletonEq in H1. rewrite H1.
+    rewrite UnionSwap. eauto. auto. }
+   {inv H5. inv H; unfoldTac; invertHyp; invThreadEq.   
+    {eapply IHspec_multistep; eauto. apply UnionEqTID in H1. invertHyp. eauto. }
+    {monoActs H0. destruct s1; simpl in *; omega. }
+    {monoActs H0. destruct s1; simpl in *; omega. }
+    {monoActs H0. destruct s1; simpl in *; omega. }
+    {monoActs H0. destruct s1; simpl in *; omega. }
+    {monoActs H0. destruct s1; simpl in *; omega. }
+   }
+  }
+Qed. 
+
+Fixpoint joinCtxts E1 E2 :=
+  match E1 with
+      | bindCtxt E M => bindCtxt (joinCtxts E E2) M
+      | handleCtxt E M => handleCtxt (joinCtxts E E2) M
+      | appCtxt E M => appCtxt (joinCtxts E E2) M
+      | appValCtxt E M => appValCtxt (joinCtxts E E2) M
+      | pairCtxt E M => pairCtxt (joinCtxts E E2) M
+      | pairValCtxt E M => pairValCtxt (joinCtxts E E2) M
+      | fstCtxt E => fstCtxt (joinCtxts E E2)
+      | sndCtxt E => sndCtxt (joinCtxts E E2)
+      | specRunCtxt E M => specRunCtxt (joinCtxts E E2) M
+      | specJoinCtxt E M => specJoinCtxt (joinCtxts E E2) M
+      | holeCtxt => E2
+  end. 
+
+Theorem notValFill : forall E e, ~ val e -> ~val (fill E e). 
+Proof.
+  induction E; intros; simpl; try solve[introsInv].
+  {intros c. inv c. apply IHE in H. contradiction. }
+  {intros c. inv c. apply IHE in H. contradiction. }
+  {auto. }
+Qed. 
+
+Theorem decomposeNotVal : forall t E e, decompose t E e -> E <> holeCtxt -> ~val t. 
+Proof.
+  intros. induction H; try solve[introsInv].
+  {intros c. inv c. contradiction. }
+  {introsInv. contradiction. }
+Qed. 
+
+Theorem decomposeFurther : forall E E' e e' e'',
+                                  ctxtWF e E -> decompose e' E' e'' -> ~ val e' ->
+                                  decompose (fill E e') (joinCtxts E E') e''.
+Proof.
+  induction E; intros. 
+  {simpl. constructor. inv H. eapply notValFill. auto. inv H. eapply IHE; eauto. }
+  {simpl. inv H. constructor. auto. apply notValFill; auto. eauto. }
+  {inv H. simpl. constructor; eauto. apply notValFill; eauto. }
+  {inv H. simpl. constructor; eauto. apply notValFill; eauto. }
+  {inv H. simpl. constructor; eauto. apply notValFill; eauto. }
+  {inv H. simpl. constructor; eauto. apply notValFill; eauto. }
+  {inv H. simpl. constructor; eauto. apply notValFill; eauto. }
+  {inv H. simpl. constructor; eauto. apply notValFill; eauto. }
+  {inv H. simpl. constructor; eauto. apply notValFill; eauto. }
+  {inv H. simpl. constructor; eauto. apply notValFill; eauto. }
+  {simpl. auto. }
+Qed. 
+
+
+Theorem joinFill : forall E1 E2 e, fill (joinCtxts E1 E2) e = fill E1 (fill E2 e). 
+Proof.
+  induction E1; intros; try solve[simpl; rewrite IHE1; eauto]. 
+  simpl. auto. 
+Qed. 
+
+Theorem simBasicStepFill : forall E e M M',
+                             ctxtWF e E -> basic_step M M' ->
+                             basic_step (fill E M) (fill E M'). 
+Admitted. 
+
+Theorem simSpecJoin' : forall H T H' T' tid tid' s2 s2' M M' s1 s1' N0 N1 E e p,              
+        spec_multistep H (tUnion T (tSingleton(tid,specStack s1 N0, s2, M)))
+                       H' (tUnion T' (tSingleton(tid,specStack s1' N0, s2, M'))) -> ~val e ->
+        spec_multistep H (tUnion T (tSingleton(tid',unlocked (wrapActs s1 N1 E e p),s2',fill E (specJoin(ret N1)M))))
+           H' (tUnion T' (tSingleton(tid',unlocked(wrapActs s1' N1 E e p),s2',fill E (specJoin(ret N1)M')))).
+Proof.
+  intros. dependent induction H0. 
+  {apply UnionEqTID in x. invertHyp. inv H. constructor. }
+  {copy x. unfoldSetEq H2. copy H. apply specStepSingleton in H2. invertHyp. 
+   assert(tIn (tUnion T0 (tSingleton x0)) x0). apply Union_intror. constructor. 
+   apply H3 in H2. inv H2. 
+   {copy H5. apply pullOut in H5. rewrite H5. unfoldTac. rewrite UnionSwap. econstructor. 
+    eapply specStepChangeUnused. eauto. unfoldTac. rewrite <- UnionSwap.
+    eapply IHspec_multistep; eauto. apply UnionSingletonEq in x; auto.  rewrite x. 
+    rewrite UnionSwap. auto. }
+   {inv H5. apply UnionEqTID in x. invertHyp. inv H; unfoldTac; invertHyp; invThreadEq.  
+    {inv H8. 
+     {econstructor. eapply SBasicStep; auto. eapply basicBeta.  
+
+Theorem decomposeFill : forall e e' e'' E E', 
+                          ctxtWF e E -> decompose e' E' e'' -> ~val e'' ->
+                          decompose (fill E e') (joinCtxts E E') e''. 
+Proof.
+  intros. induction H. 
+  {simpl. 
+
+
+
+
+
+
+
+
+
+
+
 Theorem stepWF : forall H T t H' t', 
                    wellFormed H (tUnion T t) -> step H T t (OK H' T t') ->
                    wellFormed H' (tUnion T t'). 
 Proof.
-  intros. inversion H1; subst.    
-  {destruct s1. 
+  intros. inversion H1; subst.      
+  {destruct s1.  
    {inv H0. inv H2. econstructor; eauto. rewrite unspecUnionComm in *. 
     rUnspecAll. unfoldTac. rewrite union_empty_r in *. eapply spec_multi_trans; eauto. 
     econstructor. eapply SBasicStep. eauto. constructor. constructor. } 
@@ -228,6 +382,9 @@ Proof.
     eauto. rewriteEmpty HNil. eapply SBasicStep; eauto. constructor. constructor. 
     uCons a l. eapply unspecTwoActs. eauto. }
    }
+   {inv H0. inv H2. econstructor; eauto. rewrite unspecUnionComm in *. rUnspecAll. 
+    eapply spec_multi_trans. eassumption. econstructor. eapply SBasicStep; eauto.
+    constructor. constructor. }
   }
   {inv H0. inv H2. econstructor; eauto. destruct s1.
    {simpl. unfoldTac. rewrite coupleUnion in *. repeat rewrite unspecUnionComm in *. 
@@ -249,6 +406,9 @@ Proof.
     econstructor. eapply SFork. rewrite <- coupleUnion. constructor. uCons a l.
     rewrite unspecTwoActs'. eauto. }
    }
+   {simpl. unfoldTac. rewrite coupleUnion in *. repeat rewrite unspecUnionComm in *. 
+    repeat rUnspecAll. unfoldTac. repeat rewrite union_empty_r in *. eapply spec_multi_trans.
+    eassumption. econstructor. eapply SFork. rewrite <- coupleUnion. constructor. }
   }
   {inv H0. inv H3. econstructor; eauto. erewrite unspecHeapRBRead; eauto. destruct s1.  
    {rewrite unspecUnionComm in *. simpl. rUnspecAll. unfoldTac. rewrite union_empty_r in *. 
@@ -261,6 +421,8 @@ Proof.
     erewrite unspecSingleton in H4. Focus 2. uCons a l. rewrite <- unspecTwoActs'. eauto. 
     eapply spec_multi_trans. eassumption. econstructor. eapply SGet; eauto. constructor. }
    }
+   {rewrite unspecUnionComm in *. simpl. rUnspecAll. 
+    eapply spec_multi_trans. eassumption. econstructor. eapply SGet; eauto. constructor. }
   }
   {inv H0. inv H3. econstructor; eauto. erewrite unspecHeapAddWrite; eauto. destruct s1.  
    {rewrite unspecUnionComm in *. simpl. rUnspecAll. unfoldTac. rewrite union_empty_r in *. 
@@ -273,8 +435,17 @@ Proof.
      eassumption. econstructor. eapply SPut; eauto. constructor. uCons a l.
      rewrite <- unspecTwoActs'. eauto. uCons a l. rewrite <- unspecTwoActs'; eauto. }
    }
+   {rewrite unspecUnionComm in *. simpl. rUnspecAll. eapply spec_multi_trans. 
+    eassumption. econstructor. eapply SPut; eauto. constructor. }
   }   
-  {admit.  }
+  {copy H5. unfoldTac. rewrite <- Union_associative in H0. rewrite wfFrame in H0. 
+   eapply rollbackWF in H5; eauto. Focus 2. unfold commitPool. intros. inv H3; auto.
+   econstructor; eauto. uCons (wAct x t0 E N d) (@nil action). rewrite unspecHeapAddWrite; auto. 
+   inv H5. inv H6. rewrite unspecUnionComm in H7. repeat rewrite unspecUnionComm. simpl. 
+   erewrite unspecSingleton. Focus 2. unspecThreadTac. rewrite app_nil_l. auto. 
+   unfoldTac. rewrite <- Union_associative. erewrite <- spec_multi_unused in H7. 
+   eapply spec_multi_trans. eassumption. econstructor. eapply SPut; eauto. 
+   simpl. rewrite <- Union_associative. constructor. }
   {inv H0. inv H3. econstructor; eauto. erewrite unspecHeapExtend; eauto. destruct s1. 
    {rewrite unspecUnionComm in *. simpl. rUnspecAll. unfoldTac. rewrite union_empty_r in *. 
     eapply spec_multi_trans. eassumption. copy d. apply decomposeEq in H0; subst. 
@@ -288,6 +459,9 @@ Proof.
      constructor. uCons a l. rewrite <- unspecTwoActs'. eauto. uCons a l. 
      rewrite <- unspecTwoActs'; eauto. }
    }
+   {rewrite unspecUnionComm in *. simpl. rUnspecAll. 
+    eapply spec_multi_trans. eassumption. copy d. apply decomposeEq in H0; subst. 
+    econstructor. eapply SNew; eauto. constructor. }
   }   
   {inv H0. inv H2. econstructor; eauto. destruct s1.  
    {unfoldTac. rewrite coupleUnion in *. repeat rewrite unspecUnionComm in *. simpl. 
@@ -305,8 +479,23 @@ Proof.
      rewrite union_empty_r. eapply spec_multi_trans. eassumption. econstructor. eapply SSpec. 
      rewrite <- coupleUnion. constructor. uCons a l. rewrite unspecTwoActs'. eauto. }
    }
+   {unfoldTac. rewrite coupleUnion in *. repeat rewrite unspecUnionComm in *. simpl. 
+    repeat rUnspecAll. unfoldTac. repeat rewrite union_empty_r in *. eapply spec_multi_trans. 
+    eassumption. econstructor. eapply SSpec; eauto. rewrite <- coupleUnion. constructor. }
   }
-  {admit. }   
+  {inv H0. inv H2. econstructor; eauto. unfoldTac. rewrite couple_swap in H3. 
+   rewrite coupleUnion in H3. repeat rewrite unspecUnionComm in *. 
+   erewrite unspecSingleton in H3; eauto. erewrite unspecSingleton in H3; eauto. 
+   unfoldTac. repeat rewrite <- Union_associative in H3. rewrite spec_multi_unused in H3. 
+   destructLast s1. 
+   {simpl. erewrite unspecSingleton; eauto. rewrite spec_multi_unused. unfoldTac. 
+    eapply simSpecJoin in H3. eauto. }
+   {invertHyp. eraseTrmTac (x0++[x]) M. copy H0. 
+    eapply wrapEraseTrm with(N:=N1)(E:=E)(N':=(specRun(ret N1) N0))in H0.
+    erewrite unspecSingleton. Focus 2. apply unspecEraseTrm; eauto.
+    eapply specFastForward in H3; eauto. invertHyp. eapply spec_multi_trans. 
+    eapply simTSteps in H2. eassumption. eapply simSpecJoin' in H4. simpl in *. eauto. }
+  }
   {copy H13. unfoldTac. rewrite <- Union_associative. rewrite wfFrame. Focus 2. 
    unfold commitPool. intros. inv H3. auto. rewrite <- Union_associative in H0. 
    rewrite wfFrame in H0. Focus 2. unfold commitPool; intros. inv H3. auto.
@@ -314,10 +503,12 @@ Proof.
   {inv H0. inv H2. econstructor; eauto. rewrite unspecUnionComm in *. rUnspecAll. 
    rewrite spec_multi_unused in H3. rewrite spec_multi_unused. auto. }
   {inversion H0; subst. inversion H3; subst. econstructor; eauto. erewrite unspecHeapRBRead; eauto. 
-   rewrite unspecUnionComm in *. admit. (*insert read ind here*) }
-  {admit. }
-  {admit. }
-  {admit. }
+   rewrite unspecUnionComm in *. erewrite unspecSingleton in H4. Focus 2. 
+   unspecThreadTac; auto. eraseTrmTac s1' M. erewrite unspecSingleton. Focus 2. 
+   eapply unspecEraseTrm; eauto. eapply specStepRead in H4; eauto. Focus 2. 
+   eapply lookupUnspecFull; eauto. invertHyp. rewrite unspecUnspecHeap in H2. 
+   rewrite unspecUnspecPool in H7. rewrite <- H2. inv H7. 
+   
   {inv H0. inv H2. econstructor; eauto. unfoldTac. rewrite coupleUnion in *.
    repeat rewrite unspecUnionComm in *. erewrite unspecSingleton in H3. Focus 2. 
    eapply unspecFork; auto. erewrite unspecSingleton in H3. Focus 2. 
